reduction_left

graphs/clique_to_independentSet.dfy
@@ -4,7 +4,7 @@ type Graph = (int, set<(int, int)>)
 ghost predicate validGraph(G: Graph)
     ensures forall n :: 0<n<=G.0 ==> !(exists n' :: n< n'<=n && (n, n') in G.1)
 {
-    forall u, v :: (u, v) in G.1 ==> u< v
+    forall u, v :: (u, v) in G.1 ==> 0<u< v<=G.0
 }
 
 //clique
@@ -26,10 +26,12 @@ Reduction clique->independentSet
 //reduction function
 function inverse_graph(G: Graph): Graph
     requires validGraph(G)
-    requires G.0>0
+    ensures validGraph(inverse_graph(G))
     ensures forall u, v :: 0<u< v<=G.0 ==> ((u, v) in G.1 <==> !((u, v) in inverse_graph(G).1))
+    ensures forall u, v :: 0<u< v<=G.0 ==> (!((u, v) in G.1) <==> (u, v) in inverse_graph(G).1) //necesario?
+    // ensures forall e :: e in G.1 <==> !(e in inverse_graph(G).1)    //TODO
 {
-    inverse_graph_recursive(G, G.0)
+    if G.0>0 then inverse_graph_recursive(G, G.0) else G
 }
 
 function inverse_graph_recursive(G: Graph, n: int): Graph
@@ -43,6 +45,7 @@ function inverse_graph_recursive(G: Graph, n: int): Graph
 
     ensures forall n' :: 0<n'<=n ==> (forall n'' :: n' <n''<=G.0 ==> ((n', n'') in G.1 <==> !((n', n'') in inverse_graph_recursive(G, n).1)))
     // ensures forall n' :: 0<n'<=n ==> (forall n'' :: 0<n''<=G.0 ==> ((n', n'') in G.1 <==> !((n', n'') in inverse_graph_recursive(G, n).1)))
+    // ensures forall e: (int, int) :: (0<e.0<n && e.0< e.1<=G.0) ==> (e in G.1 <==> !(e in inverse_graph_recursive(G, n).1))
 {
     if n==0 then G else
         var rG := inverse_graph_recursive(G, n-1);
@@ -129,6 +132,8 @@ function inverse_node(G: Graph, n: int, v: int): Graph
     ensures (set e | e in G.1 && 0<e.0<n) == (set e | e in inverse_node(G, n, v).1 && 0<e.0<n)
 
     ensures forall n' :: n< n'<=v ==> ((n, n') in G.1 <==> !((n, n') in inverse_node(G, n, v).1))
+    
+    // ensures forall e: (int, int) :: (e.0==n && n< e.1<=v) ==> (e in G.1 <==> !(e in inverse_node(G, n, v).1))
 {
     if v == n then G else
         var nG:= inverse_node(G, n, v-1);
@@ -137,3 +142,68 @@ function inverse_node(G: Graph, n: int, v: int): Graph
         else
             (nG.0, nG.1+{(n, v)})
 }
+
+//Reduction lemma
+lemma reduction_Lemma(G: Graph, k: nat)
+    requires validGraph(G)
+    ensures clique(G, k) <==> independentSet(inverse_graph(G), k)
+{
+    if clique(G, k)
+    {
+        reduction_Lemma_right(G, k);
+    }
+    if independentSet(inverse_graph(G), k)
+    {
+        reduction_Lemma_left(G, k);
+    }
+}
+
+lemma reduction_Lemma_right(G: Graph, k: nat)
+    requires validGraph(G)
+    requires clique(G, k)
+    ensures independentSet(inverse_graph(G), k)
+{}
+
+lemma reduction_Lemma_left(G: Graph, k: nat)
+    requires validGraph(G)
+    requires independentSet(inverse_graph(G), k)
+    ensures clique(G, k)
+{
+    inverse_graph_lemma(G);
+
+    // if k>0
+    // {
+    //     assert independentSet(inverse_graph(G), k);
+    //     assume independentSet(inverse_graph(G), k-1);   //TODO
+    //     reduction_Lemma_left(G, k-1);
+    //     assert clique(G, k-1);
+    // }
+
+    // if !clique(G, k)    //contradicción
+    // {
+    //     //!clique
+    //     assert !(exists N: set<int> :: (forall u, v :: (u in N && v in N) ==> (u, v) in G.1) && |N|==k);
+    //     //reduction function
+    //     var invG := inverse_graph(G);
+    //     assert forall u, v :: 0<u< v<=G.0 ==> ((u, v) in G.1 <==> !((u, v) in invG.1));
+    //     //independent set
+    //     assert exists N: set<int> :: (forall u, v :: (u in N && v in N) ==> !((u, v) in invG.1)) && |N|==k;
+
+    //     // ghost var iSet: set<int> :| (forall u, v :: (u in iSet && v in iSet) ==> !((u, v) in invG.1)) && |iSet| == k;    //ERROR
+
+    // }
+}
+
+lemma inverse_graph_lemma(G: Graph)
+    requires validGraph(G)
+    ensures forall e :: e in G.1 <==> !(e in inverse_graph(G).1)
+{
+    forall e | e in G.1
+    {
+        inverse_graph_local_lemma(G, e);
+    }
+}
+
+lemma inverse_graph_local_lemma(G: Graph, e: (int, int))
+    requires validGraph(G)
+    ensures e in G.1 <==> !(e in inverse_graph(G).1)
